progress

word.v
@@ -1,30 +1,85 @@
+Require Import Automata.finSet.
+
 Inductive word (char : Set) :=
   | Eps : word char
   | Concat : char -> word char -> word char.
-
-Scheme Equality for word.
-
-Parameter char : Set.
 
 Notation "'Eps'" := (Eps _).
 
 Notation "w1 ++ w2" := (Concat _ w1 w2) (at level 60, right associativity).
 
-Fixpoint length (w : word char) : nat :=
+Fixpoint length{char : Set} (w : word char) : nat :=
   match w with
   | Eps => 0
   | a ++ w' => S (length w')
   end.
 
+Definition hd{char : Set} (w : word char) :=
+match w with
+| Eps => None
+| a ++ _ => Some a
+end.
 
-Fixpoint append (w1 w2: word char) : word char :=
+Fixpoint last{char : Set} (w : word char) :=
+match w with
+| Eps => None
+| a ++ Eps => Some a
+| _ ++ t => last t
+end.
+
+Fixpoint prefix{char : Set} (w : word char) (n : nat) :=
+match n with
+| O => Eps
+| S m =>
+  match w with
+  | Eps => Eps
+  | a ++ w' => a ++ prefix w' m
+  end
+end.
+
+
+
+
+
+
+Lemma length_one_implies_head : forall (char : Set) (w : word char),
+length w > 0 -> ~ (hd w = None).
+Proof.
+  intros.
+
+  induction w.
+  simpl in H.
+  unfold not.
+  intro.
+  easy.
+  simpl.
+  discriminate.
+Qed.
+
+
+
+
+
+Fixpoint append{char : Set} (w1 w2: word char) : word char :=
   match w1 with
   | Eps => w2
   | a ++ w' => a ++ append w' w2
   end.
 
+Fixpoint exp{char : Set} (w : word char) (n : nat) :=
+match n with
+| O => Eps
+| S m => append w (exp w m)
+end.
 
-Fixpoint append_letter (w : word char) (a : char) :=
+Fixpoint exp_char{char : Set} (a : char) (n : nat) :=
+match n with
+| O => Eps
+| S m => a ++ exp_char a m
+end.
+
+
+Fixpoint append_letter{char : Set} (w : word char) (a : char) :=
   match w with
   | Eps => a ++ Eps
   | x ++ w' => x ++ append_letter w' a
@@ -34,13 +89,24 @@ Notation "w1 ** w2" := (append w1 w2) (at level 60, right associativity).
 
 Definition dlang char := word char -> Prop.
 
-Fixpoint reverse (w : word char) :=
+Fixpoint reverse{char : Set} (w : word char) :=
   match w with
   | Eps => Eps
   | a ++ w' => append_letter (reverse w') a
   end.
 
-Lemma reverse_append_is_prepend_reverse : forall (w : word char) (a : char),
+Fixpoint suffix{char : Set} (w : word char) (n : nat) :=
+let r := reverse w in
+match n with
+| O => Eps
+| S m =>
+  match w with
+  | Eps => Eps
+  | a ++ w' => a ++ suffix w' m
+  end
+end.
+
+Lemma reverse_append_is_prepend_reverse : forall (char : Set) (w : word char) (a : char),
   reverse (append_letter w a) = a ++ (reverse w).
 Proof.
   intros.
@@ -53,9 +119,11 @@ Proof.
   reflexivity.
 Qed.
 
+Definition empty {char : Set} (w : word char) := length w = O.
 
 
-Lemma reverse_involution : forall w : word char,
+
+Lemma reverse_involution : forall (char : Set) (w : word char),
   reverse (reverse w) = w.
 Proof.
   intro.
@@ -63,12 +131,37 @@ Proof.
   unfold reverse.
   reflexivity.
   simpl.
-  rewrite (reverse_append_is_prepend_reverse (reverse w) c).
+  rewrite (reverse_append_is_prepend_reverse char (reverse w) c).
   rewrite IHw.
   reflexivity.
 Qed.
 
-Definition palindrome (a : char) := { w | exists (s : word char), w = s ** (a ++ Eps) ** (reverse s)}.
+
+Fixpoint morphism {s d : Set} (h : s -> word d) (w : word s) :=
+match w with
+| Eps => Eps
+| a ++ w' => h a ** morphism h w'
+end.
+
+Fixpoint alphabetic_morphism {s d : Set} (h : s -> d) (w : word s) :=
+match w with
+| Eps => Eps
+| a ++ w' => h a ++ alphabetic_morphism h w'
+end.
 
 
+Lemma alphabetic_morphism_is_morphism : forall (s d : Set) (h : s -> d),
+  exists h' : s -> word d, forall w : word s, morphism h' w = alphabetic_morphism h w.
+Proof.
+  intros.
+  exists (fun a : s => (h a) ++ Eps).
+  intro.
+  induction w.
+  simpl.
+  reflexivity.
+  simpl.
+  rewrite IHw.
+  simpl.
+  reflexivity.
+Qed.
 
