exo.v
@@ -1,0 +1,25 @@
+Require Import Automata.word.
+
+Definition palindrome{char : Set} (a : char) : dlang char := fun w => exists (s : word char), w = s ** (a ++ Eps) ** (reverse s).
+
+Definition prefix{char : Set} (w w' : word char) := exists v : word char, (length v) > 0 /\ v ** w' = w.
+
+Definition prefixless{char : Set} (L : dlang char) : Prop :=
+  ~(exists w : word char, L w /\ (exists v, L v /\ prefix w v)).
+
+Inductive ab :=
+| a : ab
+| b : ab.
+
+Definition non_det_example (w : word ab) :=
+  exists n : nat, n > O /\ (w = exp_char a n ** exp_char b n \/ w = exp_char a n ** exp_char b (2 * n)).
+
+Inductive xyz :=
+| x : xyz
+| y : xyz
+| z : xyz.
+
+Definition non_det_example2 (w : word xyz) :=
+  exists n : nat, n > O /\ w = exp_char x n ** exp_char y n ** exp_char z n.
+
+
