pda.v
@@ -8,7 +8,7 @@ Record PDA := mkPDA {
   ; palphabet_finite : finite palphabet
   ; pstack : Set
   ; pstack_finite : finite pstack
-  ; ptransition : pstates -> pstack -> option palphabet  -> pstates -> word pstack -> Prop
+  ; ptransition : pstates -> option pstack -> option palphabet  -> pstates -> word pstack -> Prop
   ; pinitial : pstates -> Prop
   ; pfinal : pstates -> Prop
   ; pstackinitial : pstack
@@ -18,7 +18,7 @@ Record DPDA := mkDPDA {
   pda : PDA;
   determinism :
     forall q : pstates pda,
-    forall z : pstack pda,
+    forall z : option (pstack pda),
     (
       exists! comb : prod (option (palphabet pda)) (prod (pstates pda) (word (pstack pda))),
       let (a, h) := comb in
@@ -31,6 +31,63 @@ Record pconfiguration (p : PDA) := mkConfig {
   state : pstates p;
   content : word (pstack p)
 }.
+
+Definition initial_configuration{p : PDA} (c : pconfiguration p) :=
+  pinitial p (state p c).
+
+Definition final_configuration {p : PDA} (c : pconfiguration p) :=
+  pfinal p (state p c).
+
+
+Definition valid_transition_w {p : PDA} (c c' : pconfiguration p) (a : option (palphabet p)) :=
+  let '(mkConfig _ state content) := c in
+  let '(mkConfig _ state' content') := c' in
+  exists m, ptransition p state (hd content)  a state' m /\ content' = suffix content' 1 ** m.
+
+Record valid_transition {p : PDA} := mkTransition {
+  tstart : pconfiguration p;
+  tsymbol : option (palphabet p);
+  tend : pconfiguration p;
+  twittness : valid_transition_w tstart tend tsymbol
+}.
+
+Fixpoint valid_execution_w {p : PDA} (cs : word (pconfiguration p)) (letters : word (option (palphabet p))) :=
+match cs with
+| Eps => empty letters
+| c ++ Eps => True
+| c ++ c' ++ cs' =>
+  match letters with
+  | Eps => False
+  | a ++ letters' => valid_execution_w cs' letters' /\ valid_transition_w c c' a
+  end
+end.
+
+Record valid_execution (p : PDA) := mkExecution {
+  econfigurations : word (pconfiguration p);
+  eletters : word (option (palphabet p));
+  ewittness : valid_execution_w econfigurations eletters
+}.
+
+Definition accepting_execution_w (p : PDA) (e : valid_execution p) :=
+  let h := hd (econfigurations p e) in
+  let b := last (econfigurations p e) in
+  match h with
+  | None => False
+  | Some h => initial_configuration h /\
+    match b with
+    | None => False
+    | Some b => final_configuration b
+    end
+  end.
+
+Record accepting_execution (p : PDA) := mkAccExec {
+  aexecution : valid_execution p;
+  accepting : accepting_execution_w p aexecution
+}.
+
+
+
+
 
 
 
